coq/kernel/DerivedTime.v
@@ -1,0 +1,65 @@
+From Coq Require Import List Arith.PeanoNat Lia.
+
+From Kernel Require Import VMState VMStep KernelPhysics.
+From Kernel Require Import SpacetimeEmergence.
+
+Import ListNotations.
+
+Definition trace_equiv_region (s : VMState) (t1 t2 : list vm_instruction) : Prop :=
+  forall s1 s2,
+    exec_trace s t1 s1 ->
+    exec_trace s t2 s2 ->
+    forall mid, ObservableRegion s1 mid = ObservableRegion s2 mid.
+
+Definition Derived_Time (s : VMState) : Type :=
+  { t : list vm_instruction | True }.
+
+Lemma mdlacc_preserves_all_regions :
+  forall s module cost s',
+    vm_step s (instr_mdlacc module cost) s' ->
+    forall mid, ObservableRegion s mid = ObservableRegion s' mid.
+Proof.
+  intros s module cost s' Hstep mid.
+  inversion Hstep; subst; simpl.
+  unfold ObservableRegion.
+  reflexivity.
+Qed.
+
+Theorem Time_Is_Not_Fundamental :
+  forall s module cost,
+    exists s',
+      exec_trace s [] s /\
+      exec_trace s [instr_mdlacc module cost] s' /\
+      (forall mid, ObservableRegion s mid = ObservableRegion s' mid) /\
+      [] <> [instr_mdlacc module cost].
+Proof.
+  intros s module cost.
+  exists (advance_state s (instr_mdlacc module cost) (vm_graph s) (vm_csrs s) (vm_err s)).
+  split.
+  - constructor.
+  - split.
+    + eapply exec_trace_cons.
+      * apply step_mdlacc.
+      * constructor.
+    + split.
+      * intro mid.
+        apply mdlacc_preserves_all_regions with (module := module) (cost := cost).
+        apply step_mdlacc.
+      * discriminate.
+Qed.
+
+Theorem trace_equiv_region_stutter :
+  forall s module cost,
+    trace_equiv_region s [] [instr_mdlacc module cost].
+Proof.
+  intros s module cost s1 s2 Hnil Hone mid.
+  inversion Hnil; subst.
+  inversion Hone; subst.
+  repeat match goal with
+         | H : exec_trace _ [] _ |- _ => inversion H; subst; clear H
+         end.
+  match goal with
+  | Hstep : vm_step _ (instr_mdlacc _ _) _ |- _ =>
+      eapply mdlacc_preserves_all_regions; eauto
+  end.
+Qed.
