coq/thielemachine/coqproofs/DissipativeEmbedding.v
@@ -30,6 +30,8 @@ Definition encode_lattice (l : PhysLattice) : VMState :=
   {| vm_graph := {| pg_next_id := S (List.length l);
                     pg_modules := encoded_modules l |};
      vm_csrs := {| csr_cert_addr := 0; csr_status := 0; csr_err := 0 |};
+     vm_regs := repeat 0 32;
+     vm_mem := repeat 0 256;
      vm_pc := 0;
      vm_mu := 0;
      vm_err := false |}.
